Get examples working again

pulse/examples/steel/arraystructs/IntOrBool.fsti
@@ -1,75 +1,59 @@
 module IntOrBool
 
-open AggregateRef
 open FStar.PCM
-open FStar.PCM.Extras
 open FStar.PCM.POD
+open Steel.C.PCM
 open Steel.Effect
 module M = Steel.Memory
 module A = Steel.Effect.Atomic
 
 /// union int_or_bool { int i; bool b; };
 ///
-/// Carrier of PCM for int_or_bool:
+/// PCM for int_or_bool:
 
 type int_or_bool_case = | I | B
 
 let int_or_bool_cases k = match k with
   | I -> pod int
   | B -> pod bool
-let int_or_bool = union int_or_bool_cases
-
-/// PCM for int_or_bool:
-
-let int_or_bool_cases_pcm k: refined_one_pcm (int_or_bool_cases k) = match k with
+  
+let int_or_bool_cases_pcm k: pcm (int_or_bool_cases k) = match k with
   | I -> pod_pcm int
   | B -> pod_pcm bool
-  
-let int_or_bool_pcm: refined_one_pcm int_or_bool = union_pcm int_or_bool_cases_pcm
+let int_or_bool = union int_or_bool_cases_pcm
+let int_or_bool_pcm: pcm int_or_bool = union_pcm int_or_bool_cases_pcm
 
 /// (mk_int i) represents (union int_or_bool){.i = i}
 /// (mk_bool b) represents (union int_or_bool){.b = b}
 
-//val mk: tag -> Ghost.erased (int_or_bool_cases tag) -> Ghost.erased int_or_bool
-
 val mk_int (i: Ghost.erased (pod int)): Ghost.erased int_or_bool
 val mk_bool (i: Ghost.erased (pod bool)): Ghost.erased int_or_bool
 
-/// Refinements for cases
+/// Connections for cases
 
-val re_i : pcm_refinement int_or_bool_pcm
-val re_b : pcm_refinement int_or_bool_pcm
-
-/// Lenses for cases
-
-val _i : pcm_lens (refined_pcm re_i) (pod_pcm int)
-val _b : pcm_lens (refined_pcm re_b) (pod_pcm bool)
+val _i : connection int_or_bool_pcm (pod_pcm int)
+val _b : connection int_or_bool_pcm (pod_pcm bool)
 
 /// Taking pointers to the i and b cases of an int_or_bool
 
-//val addr_of_i (#i: Ghost.erased (pod int){case u == I}) (p: ref 'a int_or_bool_pcm)
-//: SteelT (q:ref 'a (pod_pcm int){q == ref_focus (ref_refine p re_i) _i})
-//    (p `pts_to` u)
-//    (fun q -> q `pts_to` proj2 u)
-
 val addr_of_i (#i: Ghost.erased (pod int)) (p: ref 'a int_or_bool_pcm)
-: SteelT (q:ref 'a (pod_pcm int){q == ref_focus (ref_refine p re_i) _i})
+: SteelT (q:ref 'a (pod_pcm int){q == ref_focus p _i})
     (p `pts_to` mk_int i)
     (fun q -> q `pts_to` i)
 
 val unaddr_of_i (#i: Ghost.erased (pod int)) (#opened: M.inames)
   (p: ref 'a int_or_bool_pcm)
-  (q: ref 'a (pod_pcm int){q == ref_focus (ref_refine p re_i) _i})
+  (q: ref 'a (pod_pcm int){q == ref_focus p _i})
 : A.SteelGhostT unit opened (q `pts_to` i) (fun _ -> p `pts_to` mk_int i)
 
 val addr_of_b (#b: Ghost.erased (pod bool)) (p: ref 'a int_or_bool_pcm)
-: SteelT (q:ref 'a (pod_pcm bool){q == ref_focus (ref_refine p re_b) _b})
+: SteelT (q:ref 'a (pod_pcm bool){q == ref_focus p _b})
     (p `pts_to` mk_bool b)
     (fun q -> q `pts_to` b)
 
 val unaddr_of_b (#b: Ghost.erased (pod bool)) (#opened: M.inames)
   (p: ref 'a int_or_bool_pcm)
-  (q: ref 'a (pod_pcm bool){q == ref_focus (ref_refine p re_b) _b})
+  (q: ref 'a (pod_pcm bool){q == ref_focus p _b})
 : A.SteelGhostT unit opened (q `pts_to` b) (fun _ -> p `pts_to` mk_bool b)
 
 /// Switching the case
